soundnessopen.v
@@ -1,14 +1,14 @@
 From WR Require Import syntax join semtypingopen normalform typing common imports.
 
-Definition γ_ok Γ γ := forall i, i < length Γ -> forall m PA, InterpUnivN m (subst_tm γ (dep_ith Γ i)) PA -> PA (γ i).
-Definition SemWt Γ a A := forall γ, γ_ok Γ γ -> exists m PA, InterpUnivN m (subst_tm γ A) PA /\ PA (subst_tm γ a).
+Definition ρ_ok Γ ρ := forall i, i < length Γ -> forall m PA, InterpUnivN m (subst_tm ρ (dep_ith Γ i)) PA -> PA (ρ i).
+Definition SemWt Γ a A := forall ρ, ρ_ok Γ ρ -> exists m PA, InterpUnivN m (subst_tm ρ A) PA /\ PA (subst_tm ρ a).
 Definition SemWff Γ := forall i, i < length Γ -> exists F, SemWt (skipn (S i) Γ) (ith Γ i) (tUniv (F i)).
 
-Lemma γ_ok_cons i Γ γ a PA A :
-  InterpUnivN i (subst_tm γ A) PA ->
+Lemma ρ_ok_cons i Γ ρ a PA A :
+  InterpUnivN i (subst_tm ρ A) PA ->
   PA a ->
-  γ_ok Γ γ ->
-  γ_ok (A :: Γ) (a .: γ).
+  ρ_ok Γ ρ ->
+  ρ_ok (A :: Γ) (a .: ρ).
 Proof.
   move => h0 h1 h2.
   case => /= [_ | m ? PA0].
@@ -16,19 +16,19 @@ Proof.
     asimpl in hPA0.
     suff : PA = PA0 by congruence.
     hauto l:on use:InterpUnivN_deterministic'.
-  - asimpl. hauto lq:on unfold:γ_ok solve+:lia.
+  - asimpl. hauto lq:on unfold:ρ_ok solve+:lia.
 Qed.
 
-Lemma γ_ok_renaming Γ γ :
+Lemma ρ_ok_renaming Γ ρ :
   forall Δ ξ,
     good_renaming ξ Γ Δ ->
-    γ_ok Δ γ ->
-    γ_ok Γ (ξ >> γ).
+    ρ_ok Δ ρ ->
+    ρ_ok Γ (ξ >> ρ).
 Proof.
   move => Δ ξ hscope h1.
-  rewrite /γ_ok => i hi j PA.
-  replace (subst_tm (ξ >> γ) (dep_ith Γ i)) with
-    (subst_tm γ (ren_tm ξ (dep_ith Γ i))); last by asimpl.
+  rewrite /ρ_ok => i hi j PA.
+  replace (subst_tm (ξ >> ρ) (dep_ith Γ i)) with
+    (subst_tm ρ (ren_tm ξ (dep_ith Γ i))); last by asimpl.
   rewrite /good_renaming in hscope.
   case /(_ i hi) : hscope => ? h0.
   rewrite -h0 => //.
@@ -41,21 +41,21 @@ Lemma renaming_SemWt Γ a A :
     good_renaming ξ Γ Δ ->
     SemWt Δ (ren_tm ξ a) (ren_tm ξ A).
 Proof.
-  rewrite /SemWt => h Δ ξ hξ γ hγ.
-  have hγ' : (γ_ok Γ (ξ >> γ)) by eauto using γ_ok_renaming.
-  case /(_ _ hγ') : h => PA hPA.
+  rewrite /SemWt => h Δ ξ hξ ρ hρ.
+  have hρ' : (ρ_ok Γ (ξ >> ρ)) by eauto using ρ_ok_renaming.
+  case /(_ _ hρ') : h => PA hPA.
   exists PA.
   by asimpl.
 Qed.
 
 Lemma SemWt_Univ Γ A i :
   SemWt Γ A (tUniv i) <->
-  forall γ, γ_ok Γ γ -> exists PA , InterpUnivN i (subst_tm γ A) PA.
+  forall ρ, ρ_ok Γ ρ -> exists PA , InterpUnivN i (subst_tm ρ A) PA.
 Proof.
   rewrite /SemWt.
   split.
   - hauto lq:on rew:off use:InterpUnivN_Univ_inv'.
-  - move => /[swap] γ /[apply].
+  - move => /[swap] ρ /[apply].
     case => PA hPA.
     exists (S i). eexists.
     split.
@@ -69,11 +69,11 @@ Theorem soundness Γ :
 Proof.
   move : Γ.
   apply wt_mutual.
-  - move => Γ i h ih ? γ hγ.
+  - move => Γ i h ih ? ρ hρ.
     move /(_ i ltac:(done)) in ih.
     case : ih => F ih.
     suff ih' : SemWt Γ (dep_ith Γ i) (tUniv (F i)).
-    + case /(_ _ hγ) : ih' => j [PA [hPA hi]].
+    + case /(_ _ hρ) : ih' => j [PA [hPA hi]].
       simpl in hPA.
       simp InterpUniv in hPA.
       move /InterpExt_Univ_inv : hPA => [? h0]; subst.
@@ -83,43 +83,43 @@ Proof.
   - hauto l:on use:SemWt_Univ.
   - move => Γ i A B _ /SemWt_Univ h0 _ /SemWt_Univ h1.
     apply SemWt_Univ.
-    move => γ hγ.
-    move /(_ γ hγ) : h0; intros (PA & hPA).
+    move => ρ hρ.
+    move /(_ ρ hρ) : h0; intros (PA & hPA).
     eexists => /=.
     apply InterpUnivN_Fun_nopf; eauto.
-    move => *; asimpl. eauto using γ_ok_cons.
-  - move => Γ A b B i _ /SemWt_Univ hB _ hb γ hγ.
-    case /(_ γ hγ) : hB => /= PPi hPPi.
+    move => *; asimpl. eauto using ρ_ok_cons.
+  - move => Γ A b B i _ /SemWt_Univ hB _ hb ρ hρ.
+    case /(_ ρ hρ) : hB => /= PPi hPPi.
     exists i, PPi. split => //.
     move /InterpUnivN_Fun_inv_nopf : hPPi.
     intros (PA & hPA & hTot & ?). subst.
     rewrite /ProdSpace.
     move => a PB ha. asimpl => hPB.
-    have : γ_ok (A :: Γ) (a .: γ) by eauto using γ_ok_cons.
+    have : ρ_ok (A :: Γ) (a .: ρ) by eauto using ρ_ok_cons.
     move /hb.
     intros (m & PB0 & hPB0 & hPB0').
     replace PB0 with PB in * by hauto l:on use:InterpUnivN_deterministic'.
     qauto l:on use:P_AppAbs_cbn,InterpUnivN_back_clos  solve+:(by asimpl).
-  - move => Γ f A B b _ ihf _ ihb γ hγ.
+  - move => Γ f A B b _ ihf _ ihb ρ hρ.
     rewrite /SemWt in ihf ihb.
-    move /(_ γ hγ) : ihf; intros (i & PPi & hPi & hf).
-    move /(_ γ hγ) : ihb; intros (j & PA & hPA & hb).
+    move /(_ ρ hρ) : ihf; intros (i & PPi & hPi & hf).
+    move /(_ ρ hρ) : ihb; intros (j & PA & hPA & hb).
     simpl in hPi.
     move /InterpUnivN_Fun_inv_nopf : hPi. intros (PA0 & hPA0 & hTot & ?). subst.
     have ? : PA0 = PA by eauto using InterpUnivN_deterministic'. subst.
     move  : hf (hb) => /[apply].
     move : hTot hb. move/[apply].
     asimpl. hauto lq:on.
-  - move => Γ a A B i _ hA _ /SemWt_Univ hB ? γ hγ.
-    have ? : Coherent (subst_tm γ A) (subst_tm γ B)
+  - move => Γ a A B i _ hA _ /SemWt_Univ hB ? ρ hρ.
+    have ? : Coherent (subst_tm ρ A) (subst_tm ρ B)
       by eauto using Coherent_subst_star.
     qauto l:on use:InterpUnivN_Coherent unfold:SemWt.
   - hauto l:on.
   - hauto l:on.
-  - move => Γ a b c A l _ /SemWt_Univ hA _ ha _ hb _ hc γ hγ.
-    case /(_ γ hγ) : ha => i [? [/InterpUnivN_Bool_inv ? ha']]; subst.
-    case /(_ γ hγ) : hb => j [PA [hPA hb']].
-    case /(_ γ hγ) : hc => k [PB [hPB hc']].
+  - move => Γ a b c A l _ /SemWt_Univ hA _ ha _ hb _ hc ρ hρ.
+    case /(_ ρ hρ) : ha => i [? [/InterpUnivN_Bool_inv ? ha']]; subst.
+    case /(_ ρ hρ) : hb => j [PA [hPA hb']].
+    case /(_ ρ hρ) : hc => k [PB [hPB hc']].
     move : ha' => [v [hred [hv|hv]]].
     + case : v hred hv => // ha0 _.
       * exists j, PA.
@@ -135,13 +135,13 @@ Proof.
         apply : InterpUnivN_back_clos_star; eauto.
         eauto using P_IfFalse_star.
     (* New case for when the scrutinee is neutral *)
-    + have ? : wne (subst_tm γ a) by hauto lq:on use:wne_if, adequacy.
-      have : γ_ok (tBool :: Γ) (subst_tm γ a .: γ). apply : (γ_ok_cons i); hauto l:on ctrs:InterpExt.
+    + have ? : wne (subst_tm ρ a) by hauto lq:on use:wne_if, adequacy.
+      have : ρ_ok (tBool :: Γ) (subst_tm ρ a .: ρ). apply : (ρ_ok_cons i); hauto l:on ctrs:InterpExt.
       move /hA => [PN hPN]. exists l, PN. split; first by asimpl.
       qauto l:on use:adequacy, wne_if unfold:CR .
   - hauto l:on use:SemWt_Univ.
   - hauto lq:on use:InterpUnivN_Univ_inv, SemWt_Univ.
-  - move => Γ a A _ _ _ ha γ.
+  - move => Γ a A _ _ _ ha ρ.
     move : ha. move/[apply]. move => [m [PA [h0 h1]]].
     exists 0. eexists.
     split => /=.
@@ -149,13 +149,13 @@ Proof.
       hauto l:on use:adequacy, InterpUniv_wn_ty, InterpUnivN_Eq unfold:CR.
     + qauto l:on ctrs:rtc use:Coherent_reflexive inv:Par .
   - move => Γ a b A i j _ ha _ hb _ /SemWt_Univ hA.
-    apply SemWt_Univ => γ hγ.
+    apply SemWt_Univ => ρ hρ.
     eexists => /=. apply InterpUnivN_Eq;
       hauto l:on use:adequacy, InterpUniv_wn_ty unfold:SemWt, CR.
-  - move => Γ t a b p A i j C _ ha _ hb _ _ _ hp _ /SemWt_Univ hC _ ht γ hγ.
-    move : hp (hγ); move/[apply] => /=. intros (m & PA & hPA & hp).
+  - move => Γ t a b p A i j C _ ha _ hb _ _ _ hp _ /SemWt_Univ hC _ ht ρ hρ.
+    move : hp (hρ); move/[apply] => /=. intros (m & PA & hPA & hp).
     move  /InterpUnivN_Eq_inv : hPA. intros (-> & ? & ? & ?).
-    move : ht (hγ); move/[apply]. intros (k & PA & hPA & ht).
+    move : ht (hρ); move/[apply]. intros (k & PA & hPA & ht).
     move : hp.
     move =>[[hp hco] | ?].
     + exists k, PA.
@@ -164,7 +164,7 @@ Proof.
         apply : InterpUnivN_Coherent; eauto.
         rewrite /Coherent.
         case : hco => ab ?.
-        exists (subst_tm (tRefl .: (ab .: γ)) C).
+        exists (subst_tm (tRefl .: (ab .: ρ)) C).
         split.
         ** apply pars_morphing_star; last by apply rtc_refl.
            apply good_pars_morphing_ext2;
@@ -173,18 +173,18 @@ Proof.
            apply good_pars_morphing_ext2. apply rtc_refl.
            tauto. apply good_pars_morphing_one.
       * asimpl.
-        eapply InterpUnivN_back_clos_star with (b := subst_tm γ t); eauto.
+        eapply InterpUnivN_back_clos_star with (b := subst_tm ρ t); eauto.
         sfirstorder use: P_JRefl_star.
     + asimpl.
-      move /(_ (subst_tm γ p .: (subst_tm γ b .: γ))) : hC.
+      move /(_ (subst_tm ρ p .: (subst_tm ρ b .: ρ))) : hC.
       case.
-      * eapply γ_ok_cons with (i := 0).
+      * eapply ρ_ok_cons with (i := 0).
         asimpl.
         apply InterpUnivN_Eq; eauto.
         right. auto.
-        move : hb (hγ). move/[apply].
+        move : hb (hρ). move/[apply].
         move => [i0 [PA0 hb0]].
-        hauto l:on use:γ_ok_cons.
+        hauto l:on use:ρ_ok_cons.
       * move => PC hPC.
         exists i, PC. split; first tauto.
         qauto l:on use:adequacy,wne_j unfold:CR.
@@ -201,7 +201,7 @@ Proof.
   elim.
   - asimpl.
     hauto l:on use:adequacy, InterpUniv_wn_ty unfold:CR.
-  - rewrite /γ_ok.
+  - rewrite /ρ_ok.
     move=> i ? m PA. asimpl.
     hauto q:on ctrs:rtc use:adequacy.
 Qed.
